theories/rust_typing/uninit_def.v
@@ -3,133 +3,64 @@ From refinedrust Require Import options.
 
 (** * Uninitialized memory *)
 
-(** This file just contains the uninit type definition (without rules), because we need it for the struct ltype definition. 
+(** This file just contains the uninit type definition (without rules), because we need it for the struct ltype definition.
   The rules are in [uninit.v]. *)
 
-(** The [bytewise] type allows to give a predicate that needs to hold for all bytes
+(** The [uninit] type allows to give a predicate that needs to hold for all bytes
   owned by the type. *)
-Section bytewise.
-  Context `{!typeGS Σ}.
-  Implicit Types P : mbyte → Prop.
-
-  Program Definition bytewise (P : mbyte → Prop) (st : syn_type) : type unit := {|
-    st_own π _ v :=
-        (∃ ly, ⌜syn_type_has_layout st ly⌝ ∗
-        ⌜v `has_layout_val` ly⌝ ∗
-        ⌜Forall P v⌝)%I;
-    st_has_op_type ot mt :=
-      ∃ ly, syn_type_has_layout st ly ∧ ot = UntypedOp ly;
-    st_syn_type := st;
-  |}.
-  Next Obligation.
-    intros. simpl. iIntros "(%ly & ? & ? & ?)"; eauto.
-  Qed.
-  Next Obligation.
-    intros ? st ot mt (ly & Hst & ->). done.
-  Qed.
-  Next Obligation.
-    simpl. iIntros (P st ot mt ? π ? v (ly & ? & ->)) "(%ly' & % & % & %)".
-    assert (ly' = ly) as ->. { by eapply syn_type_has_layout_inj. }
-    destruct mt.
-    - done.
-    - iExists ly. done.
-    - done.
-  Qed.
-
-  Global Instance bytewise_copy P st : Copyable (bytewise P st).
-  Proof. apply _. Qed.
-
-  Lemma bytewise_weaken v π P1 P2 st :
-    (∀ b, P1 b → P2 b) →
-    v ◁ᵥ{π} .@ bytewise P1 st -∗ v ◁ᵥ{π} .@ bytewise P2 st.
-  Proof.
-    iIntros (? (ly & Hst & Hly & ?)). iExists ly.
-    iPureIntro. split_and!; [done.. | ].
-    by eapply Forall_impl.
-  Qed.
-
-  Lemma bytewise_weaken_share l π κ P1 P2 st :
-    (∀ b, P1 b → P2 b) →
-    l ◁ₗ{π, κ} .@ bytewise P1 st -∗ l ◁ₗ{π, κ} .@ bytewise P2 st.
-  Proof.
-    iIntros (?) "(%v & %ly & Hb)". simpl.
-    iDestruct "Hb" as "(Hb & (%ly' & Hc) & Hd)".
-    iExists v, ly. iFrame. iNext. simpl.
-    iDestruct "Hc" as "(% & % & %)".
-    iPureIntro. eexists _. split_and!; [done.. | ].
-    by eapply Forall_impl.
-  Qed.
-
-
-  (*
-  Lemma split_bytewise v n π P ly:
-    (n ≤ ly.(ly_size))%nat →
-    v ◁ᵥ{π} .@ bytewise P ly -∗
-      (take n v) ◁ᵥ{π} .@ bytewise P (ly_set_size ly n) ∗
-      (drop n v) ◁ᵥ{π} .@ bytewise P (ly_offset ly n).
-  Proof.
-    iIntros (?[Hv HP]). iSplitL.
-    - eapply Forall_take in HP; iSplitL; last done.
-      iPureIntro. rewrite /has_layout_val in Hv.
-      by rewrite /has_layout_val length_take min_l // Hv.
-    - eapply Forall_drop in HP; iSplitL; last done.
-      iPureIntro. by rewrite /has_layout_val length_drop Hv.
-  Qed.
-  (* the corresponding lemma for shared ownership does not seem provable currently: how should we split the fractured borrow?*)
-  (* TODO: check if this is a fundamental limitation / why are fractured borrows not covariant in their predicate? *)
-
-  Lemma merge_bytewise v1 v2 π P ly1 ly2:
-    (ly1.(ly_size) ≤ ly2.(ly_size))%nat →
-    (ly_align ly2 ≤ ly_align ly1)%nat →
-    v1 ◁ᵥ{π} .@ bytewise P ly1 -∗
-    v2 ◁ᵥ{π} .@ (bytewise P (ly_offset ly2 ly1.(ly_size))) -∗
-    (v1 ++ v2) ◁ᵥ{π} .@ bytewise P ly2.
-  Proof.
-    iIntros (??) "(%Hv1 & %HP1) (%Hv2 & %HP2)".
-    iSplitL; iPureIntro.
-    - rewrite /has_layout_val length_app Hv1 Hv2.
-      rewrite {2}/ly_size/=. lia.
-    - by apply Forall_app.
-  Qed.
-  *)
-
-  (*
-     ltype Own: essentially l ↦ v st. Forall P v
-
-     if we offset l, then we get:
-      two ltype owns! one for the first part, one for the latter.
-      should pass the type of the latter on to the continuation
-
-      how do we make that compatible with ltypes?
-      -> the predicate/type we give to the continuation should be a predicate on rvalues, fundamentally.
-        (it should handle the addition of two integers which are not stored on the stack/heap, but are just temporary rvalues  without an address).
-      so, have a ltype-own to type conversion?
-
-      alternative: directly state the whole typing rule in terms of rvalue stuff, including the ownership of the p.
-        in this case: the owned ptr rvalue.
-
-      then to apply this rule in practice: need a subsumption rule for having
-        l ◁ₗ[_, Owned] r @ ◁ ty and v ◁ᵥ (r, l) @ own ty
-                                or rather v ◁ᵥ r @ own (r @ ty) ??
-  *)
-
-End bytewise.
-
-Notation "bytewise< P , st >" := (bytewise P st)
-  (only printing, format "'bytewise<' P ',' st '>'") : printing_sugar.
-
-Notation uninit := (bytewise (λ _, True)).
-
 Section uninit.
   Context `{!typeGS Σ}.
 
-  Lemma uninit_own_spec π v st :
-    (v ◁ᵥ{π} .@ uninit st)%I ≡ (∃ ly, ⌜syn_type_has_layout st ly⌝ ∗ ⌜v `has_layout_val` ly⌝)%I.
+  Program Definition uninit (st : syn_type) : type unit := {|
+    st_own π _ v :=
+        (∃ ly, ⌜syn_type_has_layout st ly⌝ ∗
+        ⌜v `has_layout_val` ly⌝)%I;
+    st_has_op_type ot mt :=
+      ∃ ly, syn_type_has_layout st ly ∧
+      match mt with
+      | MCId =>
+          ot = UntypedOp ly
+      | _ =>
+          ot_layout ot = ly
+      end;
+    st_syn_type := st;
+  |}.
+  Next Obligation.
+    intros. simpl. iIntros "(%ly & ? & ?)"; eauto.
+  Qed.
+  Next Obligation.
+    intros st ot mt (ly & Hst & ?).
+    destruct mt; subst; done.
+  Qed.
+  Next Obligation.
+    simpl. iIntros (st ot mt ? π ? v (ly & ? & Heq)) "(%ly' & % & %)".
+    assert (ly' = ly) as ->. { by eapply syn_type_has_layout_inj. }
+    destruct mt.
+    - done.
+    - subst. iExists (ot_layout ot). iPureIntro; split; first done.
+      apply has_layout_val_mem_cast. done.
+    - subst. done.
+  Qed.
+
+  Global Instance uninit_copy st : Copyable (uninit st).
+  Proof. apply _. Qed.
+
+  Lemma uninit_own_spec π v st r :
+    (v ◁ᵥ{π} r @ uninit st)%I ≡ (∃ ly, ⌜syn_type_has_layout st ly⌝ ∗ ⌜v `has_layout_val` ly⌝)%I.
   Proof.
     rewrite /ty_own_val/=; iSplit.
-    - iIntros "(%ly & ? & ? & ?)"; iExists ly. iFrame.
     - iIntros "(%ly & ? & ?)"; iExists ly. iFrame.
-      rewrite Forall_forall. done.
+    - iIntros "(%ly & ? & ?)"; iExists ly. iFrame.
+  Qed.
+
+  Lemma uninit_memcast π v r st ot hst :
+    v ◁ᵥ{π} r @ uninit st -∗
+    mem_cast v ot hst ◁ᵥ{π} r @ uninit st.
+  Proof.
+    rewrite !uninit_own_spec.
+    iIntros "(%ly & %Hst & %Hly)".
+    iExists ly. iR. iPureIntro.
+    by apply has_layout_val_mem_cast.
   Qed.
 End uninit.
 
